\documentclass[11pt, oneside]{article}
\usepackage[letterpaper, margin=2cm]{geometry}
\usepackage{MATH667}
\usepackage{booktabs}

\begin{document}
\noindent \textbf{\Large{Caleb Logemann \\
MATH667 Hyperbolic Partial Differential Equations \\
Homework 7
}}

%\lstinputlisting[language=MATLAB]{H01_23.m}
\begin{enumerate}
    \item % #1
      Derive the following 3\textsuperscript{rd} order accuracy reconstruction
      for finite volume methods.
      \begin{align*}
        u_{j+1/2}^- &= -\frac{1}{6} \bar{u}_{j-1} + \frac{5}{6}\bar{u}_j + \frac{1}{3}\bar{u}_{j+1} \\
        u_{j+1/2}^+ &= \frac{1}{3} \bar{u}_{j} + \frac{5}{6}\bar{u}_{j+1} - \frac{1}{6}\bar{u}_{j+2}
      \end{align*}

      For this problem we would like to construct a quadractic polynomial $p(x)$
      such that $p$ matches the cell average on intervals $I_{j-1}$, $I_j$, and
      $I_{j+1}$.
      If we set
      $p(x) = a\p{x - x_{j+1/2}}^2 + b\p{x - x_{j-1/2}} + c$, then
      $p(x_{j-1/2}) = c$.
      We can then solve the following three equations for $c$.
      \begin{align*}
        \frac{1}{h} \dintt{x_{j-3/2}}{x_{j-1/2}}{p(x)}{x} &= \bar{u}_{j-1} \\
        \frac{1}{h} \dintt{x_{j-1/2}}{x_{j+1/2}}{p(x)}{x} &= \bar{u}_{j} \\
        \frac{1}{h} \dintt{x_{j+1/2}}{x_{j+3/2}}{p(x)}{x} &= \bar{u}_{j+1}
      \end{align*}
      These equation can be simplified as follows.
      \begin{align*}
        \frac{1}{3h}a \p{-h^3 + 8h^3} + \frac{1}{2h}b\p{h^2 - 4h^2} + c &= \bar{u}_{j-1} \\
        \frac{1}{3h}a \p{h^3} + \frac{1}{2h}b\p{-h^2} + c &= \bar{u}_{j} \\
        \frac{1}{3h}a \p{h^3} + \frac{1}{2h}b\p{h^2} + c &= \bar{u}_{j+1}
      \end{align*}
      Simplifying gives
      \begin{align*}
        \frac{7h^2}{3}a + \frac{3h}{2}b + c &= \bar{u}_{j-1} \\
        \frac{h^2}{3}a - \frac{h}{2}b + c &= \bar{u}_{j} \\
        \frac{h^2}{3}a + \frac{h}{2}b + c &= \bar{u}_{j+1}
      \end{align*}

      %\begin{align*}
        %\frac{1}{3}a \p{x_{j-1/2}^2 + x_{j-1/2}x_{j-3/2} +  x_{j-3/2}^2} + \frac{1}{2}b\p{x_{j-1/2} + x_{j-3/2}} + c &= \bar{u}_{j-1} \\
        %\frac{1}{3}a \p{x_{j+1/2}^2 + x_{j+1/2}x_{j-1/2} +  x_{j-1/2}^2} + \frac{1}{2}b\p{x_{j+1/2} + x_{j-1/2}} + c &= \bar{u}_{j} \\
        %\frac{1}{3}a \p{x_{j+3/2}^2 + x_{j+3/2}x_{j+1/2} +  x_{j+1/2}^2} + \frac{1}{2}b\p{x_{j+3/2} + x_{j+1/2}} + c &= \bar{u}_{j+1}.
      %\end{align*}
      %Now I will substitute in so that all the x values are in terms of
      %$x_{j+1/2}$ and $h$, i.e. $x_{j-3/2} = x_{j+1/2} - 2h$,
      %$x_{j-1/2} = x_{j+1/2} - h$, etc.
      %\begin{align*}
        %\frac{1}{3}a \p{\p{x_{j+1/2} - h}^2 + \p{x_{j+1/2} - h}\p{x_{j+1/2} - 2h} +  \p{x_{j+1/2} - 2h}^2} + b\p{x_{j+1/2} - \frac{3}{2}h} + c &= \bar{u}_{j-1} \\
        %\frac{1}{3}a \p{x_{j+1/2}^2 + x_{j+1/2}\p{x_{j+1/2} - h} +  \p{x_{j+1/2} - h}^2} + b\p{x_{j+1/2} - \frac{1}{2}h} + c &= \bar{u}_{j} \\
        %\frac{1}{3}a \p{\p{x_{j+1/2} + h}^2 + \p{x_{j+1/2} + h}x_{j+1/2} +  x_{j+1/2}^2} + b\p{x_{j+1/2} + \frac{1}{2}h} + c &= \bar{u}_{j+1}.
      %\end{align*}
      %Simplifying gives
      %\begin{align*}
        %\frac{1}{3}a \p{3x_{j+1/2}^2 - 9hx_{j+1/2} + 7h^2} + b\p{x_{j+1/2} - \frac{3}{2}h} + c &= \bar{u}_{j-1} \\
        %\frac{1}{3}a \p{3x_{j+1/2}^2 - 3hx_{j+1/2} + 1h^2} + b\p{x_{j+1/2} - \frac{1}{2}h} + c &= \bar{u}_{j} \\
        %\frac{1}{3}a \p{3x_{j+1/2}^2 + 3hx_{j+1/2} + 1h^2} + b\p{x_{j+1/2} + \frac{1}{2}h} + c &= \bar{u}_{j+1}.
      %\end{align*}
      %Subtracting the last two equations and the first two equations,
      %\begin{align*}
        %-2hx_{j+1/2}a - hb &= \bar{u}_j - \bar{u}_{j+1} \\
        %\p{-2hx_{j+1/2} + 2h^2}a - hb &= \bar{u}_{j-1} - \bar{u}_{j}.
      %\end{align*}
      %Subtracting these two equations gives
      %\[
        %-2h^2a = -\bar{u}_{j-1} + 2\bar{u}_j - \bar{u}_{j+1}
      %\]
      %Solving for $a$ gives
      %\[
        %a = \frac{\bar{u}_{j-1} - 2\bar{u}_j + \bar{u}_{j+1}}{2h^2}
      %\]
      %Plugging in to the equation of $a$ and $b$, to solve for $b$ gives
      %\[
        %x_{j+1/2}\frac{-\bar{u}_{j-1} + 2\bar{u}_j - \bar{u}_{j+1}}{h} - hb = \bar{u}_j - \bar{u}_{j+1}
      %\]
      %Solving for $b$ gives
      %\[
        %b = \frac{\bar{u}_{j+1} - \bar{u}_j}{h} + x_{j+1/2}\frac{-\bar{u}_{j-1} + 2\bar{u}_j - \bar{u}_{j+1}}{h^2}
      %\]
      %Now that we have $a$ and $b$ we can solve for $c$.
      %\begin{align*}
        %\frac{1}{3}a \p{3x_{j+1/2}^2 - 3hx_{j+1/2} + 1h^2} + b\p{x_{j+1/2} - \frac{1}{2}h} + c &= \bar{u}_{j} \\
      %\end{align*}
      %\begin{align*}
        %\frac{1}{h} \dintt{x_{j-3/2}}{x_{j-1/2}}{p(x)}{x} &= \bar{u}_{j-1} \\
        %\frac{1}{h} \dintt{x_{j-1/2}}{x_{j+1/2}}{p(x)}{x} &= \bar{u}_{j} \\
        %\frac{1}{h} \dintt{x_{j+1/2}}{x_{j+3/2}}{p(x)}{x} &= \bar{u}_{j+1}
      %\end{align*}
      %These equation can be simplified as follows.
      %\begin{align*}
        %\frac{1}{3h}a \p{x_{j-1/2}^3 - x_{j-3/2}^3} + \frac{1}{2h}b\p{x_{j-1/2}^2 - x_{j-3/2}^2} + c &= \bar{u}_{j-1} \\
        %\frac{1}{3h}a \p{x_{j+1/2}^3 - x_{j-1/2}^3} + \frac{1}{2h}b\p{x_{j+1/2}^2 - x_{j-1/2}^2} + c &= \bar{u}_{j} \\
        %\frac{1}{3h}a \p{x_{j+3/2}^3 - x_{j+1/2}^3} + \frac{1}{2h}b\p{x_{j+3/2}^2 - x_{j+1/2}^2} + c &= \bar{u}_{j+1}
      %\end{align*}
      %Factoring the difference of cubes and difference of squares and cancelling
      %$h$ gives
      %\begin{align*}
        %\frac{1}{3}a \p{x_{j-1/2}^2 + x_{j-1/2}x_{j-3/2} +  x_{j-3/2}^2} + \frac{1}{2}b\p{x_{j-1/2} + x_{j-3/2}} + c &= \bar{u}_{j-1} \\
        %\frac{1}{3}a \p{x_{j+1/2}^2 + x_{j+1/2}x_{j-1/2} +  x_{j-1/2}^2} + \frac{1}{2}b\p{x_{j+1/2} + x_{j-1/2}} + c &= \bar{u}_{j} \\
        %\frac{1}{3}a \p{x_{j+3/2}^2 + x_{j+3/2}x_{j+1/2} +  x_{j+1/2}^2} + \frac{1}{2}b\p{x_{j+3/2} + x_{j+1/2}} + c &= \bar{u}_{j+1}.
      %\end{align*}
      %Now I will substitute in so that all the x values are in terms of
      %$x_{j+1/2}$ and $h$, i.e. $x_{j-3/2} = x_{j+1/2} - 2h$,
      %$x_{j-1/2} = x_{j+1/2} - h$, etc.
      %\begin{align*}
        %\frac{1}{3}a \p{\p{x_{j+1/2} - h}^2 + \p{x_{j+1/2} - h}\p{x_{j+1/2} - 2h} +  \p{x_{j+1/2} - 2h}^2} + b\p{x_{j+1/2} - \frac{3}{2}h} + c &= \bar{u}_{j-1} \\
        %\frac{1}{3}a \p{x_{j+1/2}^2 + x_{j+1/2}\p{x_{j+1/2} - h} +  \p{x_{j+1/2} - h}^2} + b\p{x_{j+1/2} - \frac{1}{2}h} + c &= \bar{u}_{j} \\
        %\frac{1}{3}a \p{\p{x_{j+1/2} + h}^2 + \p{x_{j+1/2} + h}x_{j+1/2} +  x_{j+1/2}^2} + b\p{x_{j+1/2} + \frac{1}{2}h} + c &= \bar{u}_{j+1}.
      %\end{align*}
      %Simplifying gives
      %\begin{align*}
        %\frac{1}{3}a \p{3x_{j+1/2}^2 - 9hx_{j+1/2} + 7h^2} + b\p{x_{j+1/2} - \frac{3}{2}h} + c &= \bar{u}_{j-1} \\
        %\frac{1}{3}a \p{3x_{j+1/2}^2 - 3hx_{j+1/2} + 1h^2} + b\p{x_{j+1/2} - \frac{1}{2}h} + c &= \bar{u}_{j} \\
        %\frac{1}{3}a \p{3x_{j+1/2}^2 + 3hx_{j+1/2} + 1h^2} + b\p{x_{j+1/2} + \frac{1}{2}h} + c &= \bar{u}_{j+1}.
      %\end{align*}
      %Subtracting the last two equations and the first two equations,
      %\begin{align*}
        %-2hx_{j+1/2}a - hb &= \bar{u}_j - \bar{u}_{j+1} \\
        %\p{-2hx_{j+1/2} + 2h^2}a - hb &= \bar{u}_{j-1} - \bar{u}_{j}.
      %\end{align*}
      %Subtracting these two equations gives
      %\[
        %-2h^2a = -\bar{u}_{j-1} + 2\bar{u}_j - \bar{u}_{j+1}
      %\]
      %Solving for $a$ gives
      %\[
        %a = \frac{\bar{u}_{j-1} - 2\bar{u}_j + \bar{u}_{j+1}}{2h^2}
      %\]
      %Plugging in to the equation of $a$ and $b$, to solve for $b$ gives
      %\[
        %x_{j+1/2}\frac{-\bar{u}_{j-1} + 2\bar{u}_j - \bar{u}_{j+1}}{h} - hb = \bar{u}_j - \bar{u}_{j+1}
      %\]
      %Solving for $b$ gives
      %\[
        %b = \frac{\bar{u}_{j+1} - \bar{u}_j}{h} + x_{j+1/2}\frac{-\bar{u}_{j-1} + 2\bar{u}_j - \bar{u}_{j+1}}{h^2}
      %\]
      %Now that we have $a$ and $b$ we can solve for $c$.
      %\begin{align*}
        %\frac{1}{3}a \p{3x_{j+1/2}^2 - 3hx_{j+1/2} + 1h^2} + b\p{x_{j+1/2} - \frac{1}{2}h} + c &= \bar{u}_{j} \\
      %\end{align*}
      


    \item % #2
    \item % #3

\end{enumerate}
\end{document}
